Lang.v
@@ -1,39 +1,7 @@
 From Coq Require Export Strings.String.
 From Coq Require Import Program.Equality.
 From iris.proofmode Require Import tactics.
-
-Tactic Notation "inv" ident(H) "as" simple_intropattern(ipat) :=
-  inversion H as ipat; clear H; simplify_eq.
-
-Tactic Notation "inv" ident(H) :=
-  inversion H; clear H; simplify_eq.
-
-Inductive bin_op :=
-  | PlusOp
-  | MinusOp
-  | LeOp
-  | LtOp
-  | EqOp.
-
-Inductive val :=
-  | VUnit : val
-  | VBool : bool -> val
-  | VNat : nat -> val
-  | VRef : nat -> val
-  | VPair : val -> val -> val
-  | VLock : bool -> val.
-
-Lemma val_eq_dec (v v' : val) :
-  v = v' \/ v ≠ v'.
-Proof.
-  dependent induction v; destruct v'; eauto.
-  1, 5: destruct b; destruct b0; eauto.
-  1, 2: destruct (Nat.eq_dec n n0);
-    try (left; by f_equal);
-    right; intros Heq; simplify_eq.
-  destruct (IHv1 v'1); destruct (IHv2 v'2); simplify_eq;
-  try (by left); right; intros Heq; simplify_eq.
-Qed.
+Require Import val.
 
 Inductive expr :=
   | EVal : val -> expr
@@ -79,32 +47,6 @@ Fixpoint subst (x : string) (w : val) (e : expr) : expr :=
   | EUnlock e => EUnlock (subst x w e)
   end.
 
-Definition option_and (v1 v2 : option val) : option val :=
-  match v1 with
-  | Some (VBool b1) =>
-      match v2 with
-      | Some (VBool b2) => Some (VBool (andb b1 b2))
-      | _ => None
-      end
-  | _ => None
-  end.
-
-Fixpoint eval_bin_op (op : bin_op) (v1 v2 : val) : option val :=
-  match op, v1, v2 with
-  | PlusOp, VNat n1, VNat n2 => Some (VNat (n1 + n2))
-  | MinusOp, VNat n1, VNat n2 => Some (VNat (n1 - n2))
-  | LeOp, VNat n1, VNat n2 => Some (VBool (Nat.leb n1 n2))
-  | LtOp, VNat n1, VNat n2 => Some (VBool (Nat.ltb n1 n2))
-  | EqOp, VUnit, VUnit => Some (VBool true)
-  | EqOp, VBool n1, VBool n2 => Some (VBool (Bool.eqb n1 n2))
-  | EqOp, VNat n1, VNat n2 => Some (VBool (Nat.eqb n1 n2))
-  | EqOp, VRef l1, VRef l2 => Some (VBool (Nat.eqb l1 l2))
-  | EqOp, VPair p1 p2, VPair q1 q2 =>
-      option_and (eval_bin_op EqOp p1 q1) (eval_bin_op EqOp p2 q2)
-  | EqOp, VLock b1, VLock b2 => Some (VBool (Bool.eqb b1 b2))
-  | _, _, _ => None
-  end.
-
 (* Small steps that don't alter the heap *)
 Inductive pure_step : expr -> expr -> Prop :=
   | Amb_step n : pure_step EAmb (EVal (VNat n))
@@ -129,17 +71,6 @@ Inductive pure_step : expr -> expr -> Prop :=
       pure_step (ESeq (EVal v) e) e
   | Par_step v1 v2 :
       pure_step (EPar (EVal v1) (EVal v2)) (EVal (VPair v1 v2)).
-
-(* Either a value or reserved (previously freed)
-   Corresponds to memory locations *)
-Inductive cell :=
-  | Value : val -> cell
-  | Reserved : cell.
-
-(* A heap maps a natural number to a memory location *)
-Notation heap := (gmap nat cell).
-
-Definition valid_alloc (h : heap) (n : nat) := ∀ c, h !! n = Some c → c = Reserved.
 
 Inductive head_step : expr -> heap -> expr -> heap -> Prop :=
   | do_pure_step e e' h :
@@ -270,8 +201,6 @@ Global Hint Resolve head_step_step : headstep.
 Global Hint Constructors head_step : headstep.
 Global Hint Constructors pure_step : headstep.
 
-Infix "###" := map_disjoint (at level 70).
-
 Lemma step_heap_mono e m e' m' x :
   step e m e' m' → m' ### x → m ### x.
 Proof.
@@ -373,180 +302,3 @@ Definition is_lock (e : expr) :=
     | EUnlock _ => True
     | _ => False
   end.
-
-Declare Scope S.
-Delimit Scope S with S.
-
-Definition iProp := heap → Prop.
-
-Bind Scope S with iProp.
-
-Definition iEntails (P Q : iProp) : Prop := ∀ m, P m → Q m.
-Definition iEmp : iProp := λ m, m = ∅.
-Definition iPoints (l : nat) (v : val) : iProp := λ m, m = {[ l := (Value v) ]}.
-Definition iNegPoints (l : nat) : iProp := λ m, m = {[ l := Reserved ]}.
-Definition iSep (P Q : iProp) : iProp := λ m, ∃ m1 m2, P m1 ∧ Q m2 ∧ m = m1 ∪ m2 ∧ m1 ### m2 .
-Definition iWand (P Q : iProp) : iProp := λ m, ∀ m', m ### m' → P m' → Q (m' ∪ m).
-Definition iTrue : iProp := λ m , True.
-Definition iAnd (P Q : iProp) : iProp := λ m, P m ∧ Q m.
-Definition iOr (P Q : iProp) : iProp := λ m, P m ∨ Q m.
-Definition iForall {A} (P : A → iProp) : iProp := λ m, ∀ x, P x m.
-Definition iExists {A} (P : A → iProp) : iProp := λ m, ∃ x, P x m.
-Definition iPure (φ : Prop) : iProp := λ m, φ ∧ m = ∅.
-Definition iOwn (m : heap) : iProp := λ m', m' = m.
-
-Notation "P ⊢ Q" := (iEntails P%S Q%S) (at level 99, Q at level 200).
-Notation "P ∗ Q" := (iSep P%S Q%S) (at level 80, right associativity) : S.
-Notation "P ∧ Q" := (iAnd P%S Q%S) (at level 80, right associativity) : S.
-Notation "P ∨ Q" := (iOr P%S Q%S) (at level 85, right associativity) : S.
-Notation "l ↦ v" := (iPoints l v) (at level 20) : S.
-Notation "l ↦ ⊥" := (iNegPoints l) (at level 20) : S.
-Notation "'emp'" := iEmp : S.
-Notation "P -∗ Q" := (iWand P%S Q%S) (at level 99, Q at level 200, right associativity) : S.
-Notation "@[ p ]" := (iPure p) (at level 1, p at level 200) : S.
-Notation "∀ x1 .. xn , P" :=
-  (iForall (fun x1 => .. (iForall (fun xn => P%S)) ..))
-  (at level 200, x1 binder, xn binder, right associativity) : S.
-Notation "∃ x1 .. xn , P" :=
-  (iExists (fun x1 => .. (iExists (fun xn => P%S)) ..))
-  (at level 200, x1 binder, xn binder, right associativity) : S.
-
-Ltac iUnfold := unfold iEmp, iNegPoints, iPoints, iSep, iWand, iForall, iExists, iPure, iEntails, iAnd, iOr, iTrue in *.
-
-Section seplogic.
-
-  Ltac duh := iUnfold;
-    naive_solver (
-      rewrite ?map_union_assoc ?left_id ?right_id;
-      simplify_map_eq;
-      try apply map_union_comm;
-      solve_map_disjoint).
-
-  Lemma iEntails_refl P : P ⊢ P.
-  Proof. duh. Qed.
-
-  Lemma iEntails_trans Q P R : (P ⊢ Q) → (Q ⊢ R) → (P ⊢ R).
-  Proof. duh. Qed.
-
-  Lemma iSep_mono_l P₁ P₂ Q : (P₁ ⊢ P₂) → P₁ ∗ Q ⊢ P₂ ∗ Q.
-  Proof. duh. Qed.
-
-  Lemma iSep_comm P Q : P ∗ Q ⊢ Q ∗ P.
-  Proof. duh. Qed.
-
-  Lemma iSep_assoc P Q R : P ∗ (Q ∗ R) ⊢ (P ∗ Q) ∗ R.
-  Proof. duh. Qed.
-
-  Lemma iSep_emp_l P : P ⊢ emp ∗ P.
-  Proof. duh. Qed.
-
-  Lemma iSep_emp_l_inv P : emp ∗ P ⊢ P.
-  Proof. duh. Qed.
-
-  Lemma iWand_intro_r P Q R : (P ∗ Q ⊢ R) → P ⊢ Q -∗ R.
-  Proof. duh. Qed.
-
-  Lemma iWand_elim P Q : P ∗ (P -∗ Q) ⊢ Q.
-  Proof. duh. Qed.
-
-  Lemma iAnd_intro (P Q R : iProp) : (R ⊢ P) → (R ⊢ Q) → R ⊢ P ∧ Q.
-  Proof. duh. Qed.
-
-  Lemma iAnd_elim_l (P Q : iProp) : P ∧ Q ⊢ P.
-  Proof. duh. Qed.
-
-  Lemma iAnd_elim_r (P Q : iProp) : P ∧ Q ⊢ Q.
-  Proof. duh. Qed.
-
-  Lemma iOr_intro_l (P Q : iProp) : P ⊢ P ∨ Q.
-  Proof. duh. Qed.
-
-  Lemma iOr_intro_r (P Q : iProp) : Q ⊢ P ∨ Q.
-  Proof. duh. Qed.
-
-  Lemma iOr_elim (P Q R : iProp) : (P ⊢ R) → (Q ⊢ R) → P ∨ Q ⊢ R.
-  Proof. duh. Qed.
-
-  Lemma iForall_intro {A} P (Q : A → iProp) : (∀ x, P ⊢ Q x) → (P ⊢ ∀ x, Q x).
-  Proof. duh. Qed.
-
-  Lemma iForall_elim {A} (P : A → iProp) x : (∀ z, P z) ⊢ P x.
-  Proof. duh. Qed.
-
-  Lemma iExists_intro {A} (P : A → iProp) x : P x ⊢ ∃ z, P z.
-  Proof. duh. Qed.
-
-  Lemma iExists_elim {A} (P : A → iProp) Q :  (∀ x, P x ⊢ Q) → (∃ z, P z) ⊢ Q.
-  Proof. duh. Qed.
-
-  Lemma iSep_emp_r P : P ⊢ P ∗ emp.
-  Proof. duh. Qed.
-
-  Lemma iSep_emp_r_inv P : P ∗ emp ⊢ P.
-  Proof. duh. Qed.
-
-  Lemma iSep_mono_r P Q₁ Q₂ : (Q₁ ⊢ Q₂) → P ∗ Q₁ ⊢ P ∗ Q₂.
-  Proof. duh. Qed.
-
-  Lemma iSep_mono P₁ P₂ Q₁ Q₂ : (P₁ ⊢ P₂) → (Q₁ ⊢ Q₂) → P₁ ∗ Q₁ ⊢ P₂ ∗ Q₂.
-  Proof. duh. Qed.
-
-  Lemma iSep_assoc' P Q R : (P ∗ Q) ∗ R ⊢ P ∗ (Q ∗ R).
-  Proof. intros ? (? & ? & (? & ? & ?) & ?); repeat eexists; duh. Qed.
-
-  Lemma iWand_intro_l P Q R : (Q ∗ P ⊢ R) → P ⊢ Q -∗ R.
-  Proof. duh. Qed.
-
-  Lemma iExists_sep {A} (P : A → iProp) Q : (∃ x, P x) ∗ Q ⊢ ∃ x, P x ∗ Q.
-  Proof. duh. Qed.
-
-  Lemma iPure_intro (φ : Prop) : φ → emp ⊢ @[ φ ].
-  Proof. duh. Qed.
-
-  Lemma iPure_intro' (φ : Prop) P : φ → P ⊢ @[ φ ] ∗ P.
-  Proof. duh. Qed.
-
-  Lemma iPure_elim (φ : Prop) P Q : (φ → P ⊢ Q) → @[ φ ] ∗ P ⊢ Q.
-  Proof. duh. Qed.
-
-  Lemma iPure_elim' (φ : Prop) Q : (φ → emp ⊢ Q) → @[ φ ] ⊢ Q.
-  Proof. duh. Qed.
-
-  Lemma iOr_distr (P Q R : iProp) : (P ∨ Q) ∗ R ⊢ (P ∗ R) ∨ (Q ∗ R).
-  Proof. duh. Qed.
-
-  Lemma iOr_distr' (P Q R : iProp) : (P ∗ R) ∨ (Q ∗ R) ⊢ (P ∨ Q) ∗ R.
-  Proof. duh. Qed.
-
-End seplogic.
-
-Create HintDb seplogic.
-
-Global Hint Resolve iEntails_refl : seplogic.
-Global Hint Resolve iSep_mono_l : seplogic.
-Global Hint Resolve iSep_comm : seplogic.
-Global Hint Resolve iSep_assoc : seplogic.
-Global Hint Resolve iSep_emp_l : seplogic.
-Global Hint Resolve iSep_emp_l_inv : seplogic.
-Global Hint Resolve iWand_intro_r : seplogic.
-Global Hint Resolve iWand_elim : seplogic.
-Global Hint Resolve iAnd_intro : seplogic.
-Global Hint Resolve iAnd_elim_l : seplogic.
-Global Hint Resolve iAnd_elim_r : seplogic.
-Global Hint Resolve iOr_intro_l : seplogic.
-Global Hint Resolve iOr_intro_r : seplogic.
-Global Hint Resolve iOr_elim : seplogic.
-Global Hint Resolve iForall_intro : seplogic.
-Global Hint Resolve iForall_elim : seplogic.
-Global Hint Resolve iExists_intro : seplogic.
-Global Hint Resolve iExists_elim : seplogic.
-Global Hint Resolve iSep_emp_r : seplogic.
-Global Hint Resolve iSep_emp_r_inv : seplogic.
-Global Hint Resolve iSep_mono_r : seplogic.
-Global Hint Resolve iSep_mono iSep_assoc' : seplogic.
-Global Hint Resolve iWand_intro_l : seplogic.
-Global Hint Resolve iExists_sep : seplogic.
-Global Hint Resolve iPure_intro : seplogic.
-Global Hint Resolve iPure_intro' : seplogic.
-Global Hint Resolve iPure_elim : seplogic.
-Global Hint Resolve iPure_elim' : seplogic.
