perm.v
@@ -3,11 +3,11 @@ From Coq Require Import Lists.List.
 From Coq Require Import Program.Equality.
 From Coq Require Import Bool.DecBool.
 From iris.proofmode Require Import tactics.
-Require Import Lang.
+Require Export val.
 
 Inductive base_event :=
-  | Lock : val -> base_event
-  | Unlock : val -> base_event
+  | Lock : nat -> base_event
+  | Unlock : nat -> base_event
   | Join : base_event.
 
 Inductive event :=
@@ -15,24 +15,11 @@ Inductive event :=
   | Left : event -> event
   | Right : event -> event.
 
-Lemma base_event_eq_dec (a b : base_event) :
-  a = b \/ a ≠ b.
-Proof.
-  destruct a; destruct b; eauto;
-  destruct (val_eq_dec v v0);
-  try (left; by f_equal);
-  right; intros Heq; simplify_eq.
-Qed.
+Global Instance base_event_eq_dec : EqDecision base_event.
+Proof. solve_decision. Defined.
 
-Lemma event_eq_dec (a b : event) :
-  a = b \/ a ≠ b.
-Proof.
-  dependent induction a;
-  [destruct b0 | destruct b..]; eauto;
-  [destruct (base_event_eq_dec b0 b) | destruct (IHa b)..];
-  try (left; by f_equal);
-  right; intros Heq; simplify_eq.
-Qed.
+Global Instance event_eq_dec : EqDecision event.
+Proof. solve_decision. Defined.
 
 Definition trace : Type := list event.
 
@@ -84,10 +71,8 @@ Inductive perm : trace -> trace -> Prop :=
       perm t t''.
 
 Create HintDb perm.
-Global Hint Resolve can_swap_symm : perm.
-Global Hint Resolve can_swap_irreflexive : perm.
-Global Hint Constructors perm1 : perm.
-Global Hint Constructors perm : perm.
+Global Hint Resolve can_swap_symm can_swap_irreflexive : perm.
+Global Hint Constructors perm1 perm : perm.
 
 Lemma perm_trans t t' t'' :
   perm t t' ->
@@ -228,10 +213,7 @@ Proof.
   eauto 6 with perm.
 Qed.
 
-Global Hint Resolve perm_refl : perm.
-Global Hint Resolve perm_skip : perm.
-Global Hint Resolve perm_swap : perm.
-Global Hint Resolve perm_symm : perm.
+Global Hint Resolve perm_refl perm_skip perm_swap perm_symm : perm.
 
 Lemma perm_can_swap_all a t t' :
   Forall (can_swap a) t ->
@@ -463,3 +445,285 @@ Proof.
   induction t; intros Hperm; [done|].
   apply IHt. by eapply perm_inv.
 Qed.
+
+(**************************
+    Language definition
+**************************)
+
+Notation lock_heap := (gmap nat bool).
+
+Inductive expr :=
+  | EVal : val -> expr
+  | EAmb : expr
+  | EVar : string -> expr
+  | EPair : expr -> expr -> expr
+  | EFst : expr -> expr
+  | ESnd : expr -> expr
+  | ELet : string -> expr -> expr -> expr
+  | EOp : bin_op -> expr -> expr -> expr
+  | EIf : expr -> expr -> expr -> expr
+  | EWhile : expr -> expr -> expr
+  | ESeq : expr -> expr -> expr
+  | EPar : expr -> expr -> expr
+  | ENewlock : expr
+  | ELock : expr -> expr
+  | EUnlock : expr -> expr.
+
+Fixpoint subst (x : string) (w : val) (e : expr) : expr :=
+  match e with
+  | EVal _ => e
+  | EAmb => EAmb
+  | EVar y => if string_dec y x then EVal w else EVar y
+  | EPair e1 e2 => EPair (subst x w e1) (subst x w e2)
+  | EFst e' => EFst (subst x w e')
+  | ESnd e' => ESnd (subst x w e')
+  | ELet y e1 e2 => if string_dec x y
+     then ELet y (subst x w e1) e2
+     else ELet y (subst x w e1) (subst x w e2)
+  | EOp op e1 e2 => EOp op (subst x w e1) (subst x w e2)
+  | EIf e1 e2 e3 => EIf (subst x w e1) (subst x w e2) (subst x w e3)
+  | EWhile e1 e2 => EWhile (subst x w e1) (subst x w e2)
+  | ESeq e1 e2 => ESeq (subst x w e1) (subst x w e2)
+  | EPar e1 e2 => EPar (subst x w e1) (subst x w e2)
+  | ENewlock => ENewlock
+  | ELock e => ELock (subst x w e)
+  | EUnlock e => EUnlock (subst x w e)
+  end.
+
+(* Small steps that don't alter the heap *)
+Inductive pure_step : expr -> expr -> Prop :=
+  | Amb_step n : pure_step EAmb (EVal (VNat n))
+  | Pair_step v1 v2 :
+      pure_step (EPair (EVal v1) (EVal v2)) (EVal (VPair v1 v2))
+  | Fst_step v1 v2 :
+      pure_step (EFst (EVal (VPair v1 v2))) (EVal v1)
+  | Snd_step v1 v2 :
+      pure_step (ESnd (EVal (VPair v1 v2))) (EVal v2)
+  | Let_step y e v :
+      pure_step (ELet y (EVal v) e) (subst y v e)
+  | Op_step op v1 v2 v3 :
+      eval_bin_op op v1 v2 = Some v3 ->
+      pure_step (EOp op (EVal v1) (EVal v2)) (EVal v3)
+  | If_true_step e1 e2 :
+      pure_step (EIf (EVal (VBool true)) e1 e2) e1
+  | If_false_step e1 e2 :
+      pure_step (EIf (EVal (VBool false)) e1 e2) e2
+  | While_step e1 e2 :
+      pure_step (EWhile e1 e2) (EIf e1 (ESeq e2 (EWhile e1 e2)) (EVal VUnit))
+  | Seq_step v e :
+      pure_step (ESeq (EVal v) e) e
+  | Par_step v1 v2 :
+      pure_step (EPar (EVal v1) (EVal v2)) (EVal (VPair v1 v2)).
+
+Inductive head_step : expr -> lock_heap -> expr -> lock_heap -> Prop :=
+  | do_pure_step e e' h :
+      pure_step e e' ->
+      head_step e h e' h
+  | Newlock_headstep (h : lock_heap) l :
+      l ∉ dom (gset nat) h ->
+      head_step ENewlock h (EVal (VRef l)) (<[ l := false ]> h)
+  | Lock_headstep h l :
+      h !! l = Some (false) ->
+      head_step (ELock (EVal (VRef l))) h (EVal VUnit) (<[ l := true ]> h)
+  | Unlock_headstep h l :
+      h !! l = Some (true) ->
+      head_step (EUnlock (EVal (VRef l))) h (EVal VUnit) (<[ l := false ]> h).
+
+Inductive ctx1 : (expr -> expr) -> Prop :=
+  | Pair_l_ctx e : ctx1 (fun x => EPair x e)
+  | Pair_r_ctx v : ctx1 (EPair (EVal v))
+  | Fst_ctx : ctx1 EFst
+  | Snd_ctx : ctx1 ESnd
+  | Let_ctx y e : ctx1 (fun x => ELet y x e)
+  | Op_l_ctx op e : ctx1 (fun x => EOp op x e)
+  | Op_r_ctx op v : ctx1 (fun x => EOp op (EVal v) x)
+  | If_ctx e1 e2 : ctx1 (fun x => EIf x e1 e2)
+  | Seq_ctx e : ctx1 (fun x => ESeq x e)
+  | Par_l_ctx e : ctx1 (fun x => EPar x e)
+  | Par_r_ctx e : ctx1 (EPar e)
+  | Lock_ctx : ctx1 ELock
+  | Unlock_ctx : ctx1 EUnlock.
+
+Inductive ctx : (expr -> expr) -> Prop :=
+  | Id_ctx : ctx (fun x => x)
+  | Compose_ctx k1 k2 : ctx1 k1 -> ctx k2 -> ctx (fun x => k1 (k2 x)).
+
+Lemma Single_ctx k : ctx1 k -> ctx k.
+Proof.
+  intros Hk. apply Compose_ctx; [done | constructor].
+Qed.
+
+Create HintDb context.
+Global Hint Resolve Single_ctx : context.
+Global Hint Constructors ctx1 ctx : context.
+
+Ltac inv_ctx := repeat
+  match goal with
+  | H : ctx1 _ |- _ => inv H; try done
+  | H : ctx _ |- _ => inv H; try done
+  end.
+
+Lemma context_EVal k e v :
+  ctx k -> 
+  k e = EVal v ->
+  k = (fun x => x) /\ e = EVal v.
+Proof.
+  intros Hk. induction Hk; [done|].
+  intros Hk12. inv H.
+Qed.
+
+Inductive step : expr -> lock_heap -> expr -> lock_heap -> Prop :=
+  | do_step k e e' h h' :
+      ctx k ->
+      head_step e h e' h' ->
+      step (k e) h (k e') h'.
+
+Inductive steps : expr -> lock_heap -> expr -> lock_heap -> Prop :=
+  | steps_refl e h :
+      steps e h e h
+  | steps_step e1 h1 e2 h2 e3 h3 :
+      step e1 h1 e2 h2 ->
+      steps e2 h2 e3 h3 ->
+      steps e1 h1 e3 h3.
+
+Lemma head_step_step e e' h h' :
+  head_step e h e' h' -> step e h e' h'.
+Proof.
+  intros Hhead.
+  apply (do_step (fun x => x)).
+  - repeat constructor.
+  - assumption.
+Qed.
+
+Lemma step_context_step e e' h h' k :
+  ctx k ->
+  step e h e' h' ->
+  step (k e) h (k e') h'.
+Proof.
+  intros Hctx Hstep. induction Hctx; [done|].
+  inv IHHctx. apply (do_step (fun x => (k1 (k x)))); [|done].
+  by apply Compose_ctx.
+Qed.
+
+Lemma steps_context_steps e e' h h' k :
+  ctx k ->
+  steps e h e' h' ->
+  steps (k e) h (k e') h'.
+Proof.
+  intros Hctx Hsteps.
+  induction Hsteps; [apply steps_refl |].
+  apply steps_step with (k e2) h2; [|done].
+  by apply step_context_step.
+Qed.
+
+Lemma step_once e h e' h' :
+  step e h e' h' -> steps e h e' h'.
+Proof.
+  intros Hstep.
+  econstructor; [done | constructor].
+Qed.
+
+Create HintDb headstep.
+Global Hint Resolve step_once head_step_step : headstep.
+Global Hint Constructors head_step pure_step : headstep.
+
+Lemma step_heap_mono e m e' m' x :
+  step e m e' m' → m' ### x → m ### x.
+Proof.
+  intros []?. destruct H; 
+  inv H0; try assumption;
+  rewrite map_disjoint_insert_l in H1;
+  by destruct H1.
+Qed.
+
+Lemma steps_heap_mono e m e' m' x :
+  steps e m e' m' → m' ### x -> m ### x.
+Proof.
+  induction 1; eauto using step_heap_mono.
+Qed.
+
+Lemma steps_trans e1 e2 e3 h1 h2 h3 :
+  steps e1 h1 e2 h2 -> steps e2 h2 e3 h3 -> steps e1 h1 e3 h3.
+Proof.
+  intros H1 H2.
+  induction H1; [done|].
+  eauto using steps_step.
+Qed.
+
+Lemma steps_context e k v v' h1 h2 h3 :
+  ctx k ->
+  steps e h1 (EVal v') h2 ->
+  steps (k (EVal v')) h2 (EVal v) h3 ->
+  steps (k e) h1 (EVal v) h3.
+Proof.
+  intros Hctx Hsteps1 Hsteps2.
+  induction Hsteps1; [done|].
+  eapply steps_step.
+  - apply step_context_step; done.
+  - by apply IHHsteps1.
+Qed.
+
+Lemma head_step_frame_equiv e m e' m' :
+  head_step e m e' m' <-> ∀ mf, m' ### mf -> head_step e (m ∪ mf) e' (m' ∪ mf).
+Proof.
+  split.
+  1: {
+    intros. destruct H; rewrite -? insert_union_l; try by econstructor; eauto;
+    try apply lookup_union_Some_l; eauto. constructor.
+    rewrite elem_of_dom lookup_union_is_Some. rewrite elem_of_dom in H.
+    rewrite map_disjoint_insert_l eq_None_not_Some in H0.
+    tauto.
+  }
+  intros. specialize (H ∅). rewrite !right_id in H.
+  apply H. solve_map_disjoint.
+Qed.
+
+Lemma step_frame_equiv e m e' m' :
+  step e m e' m'  ↔ ∀ mf, m' ### mf -> step e (m ∪ mf) e' (m' ∪ mf).
+Proof.
+  split.
+  - intros []. rewrite head_step_frame_equiv in H0.
+    eauto using step.
+  - intros. specialize (H _ (map_disjoint_empty_r _)).
+    by rewrite !right_id_L in H.
+Qed.
+
+Lemma steps_frame_equiv e h e' h' :
+  steps e h e' h' ↔ ∀ hf, h' ### hf → steps e (h ∪ hf) e' (h' ∪ hf).
+Proof.
+  split.
+  - induction 1; eauto using steps.
+    intros.
+    assert (h2 ### hf). { eapply steps_heap_mono; eauto. }
+    rewrite step_frame_equiv in H.
+    eapply steps_step; eauto.
+  - intros. specialize (H _ (map_disjoint_empty_r _)).
+    by rewrite !right_id_L in H.
+Qed.
+
+Definition is_val (e : expr) :=
+  match e with
+    | EVal _ => True
+    | _ => False
+  end.
+
+Lemma not_is_val_ctx1 e k :
+  ctx1 k -> ¬ is_val (k e).
+Proof.
+  intros Hctx Hnval.
+  by inv Hctx.
+Qed.
+
+Lemma not_is_val_context e k :
+  ctx k -> ¬ is_val e -> ¬ is_val (k e).
+Proof.
+  intros Hctx. generalize e. induction Hctx; intros e' Hnval;
+  [done | destruct H; easy].
+Qed.
+
+Definition is_lock (e : expr) :=
+  match e with
+    | ELock _ => True
+    | EUnlock _ => True
+    | _ => False
+  end.
